\subsection*{2.2}

\textbf{In each of the following find the PDF of Y}

\noindent \textbf{Key Theorems}

\begin{theorem}[2.1.5]
	\[f_Y(y) = \begin{cases}
		f_X(g^{-1}(y)) \cdot \left| \frac{d}{dy} g^{-1}(y) \right| & y \in \mathcal{Y} \\
		0 & o/w
	\end{cases}\]
\end{theorem}

\subsubsection*{Part A}

\textbf{NOTE:} I know Part A wasn't assigned but I did it on accident and want to save my work for future studying.

$Y = X^2$

$f_X(x) = 1; \; 0 < x < 1$

To apply theorem 2.1.5 we need a few components. The range of $Y$, the map from y to x, $g^{-1}(y)$, and the derivative of that map. 

Due to the domain of $x$ we and how $x^2$ transforms it: $\mathcal{Y} = (0,1)$.

\noindent Next, find $g^{-1}(y)$:

\begin{align*}
	x^2 &= y \\
	x &= \sqrt{y} \\
	g^{-1}(y) &= \sqrt{y}
\end{align*}

\noindent Derivative of $g^{-1}(y)$:

\begin{align*}
	\frac{d}{dy} g^{-1}(y) &= \frac{d}{dy} \sqrt{y} \\
	&= \frac{1}{2\sqrt{y}}
\end{align*}

\noindent Put it all together:

\begin{align*}
	f_X(g^{-1}(y)) \cdot \left|\frac{d}{dy} g^{-1}(y) \right| &= 1 \cdot \left| \frac{1}{2\sqrt{y}} \right| \\
	&= \frac{1}{2\sqrt{y}}
\end{align*}

\[
	f_Y(y) = \begin{cases}
		\frac{1}{2\sqrt{y}} & 0 < y < 1 \\
		0 & o/w
	\end{cases}
\]


\subsubsection*{Part B}

\begin{align*}
	Y &= -log(X) \\
	f_X(x) &= \frac{(n+m+1)!}{n!m!}x^n(1-x)^m \\
	0<x<1 ;& \; m,n \; \text{are positive integers}
\end{align*}

\noindent Solve for $g^{-1}(y)$

\begin{align*}
	y &= -log(x) \\
	-y &= log(x) \\
	e^{-y} &= x \\
	e^{-y} &= g^{-1}(y)
\end{align*}

\noindent Take derivative of $g^{-1}(y)$

\begin{align*}
	\frac{d}{dy} g^{-1}(y) &= \frac{d}{dy} e^{-y} \\
	&= -e^{-y}
\end{align*}

\noindent Put it all together

\[
	f_Y(y) = \begin{cases}
		\frac{(n+m+1)!}{n!m!} e^{-yn} \cdot (1 - e^{-y}) & 0 < y < 1 \\
		0 & o/w
	\end{cases}
\]

\pagebreak

\subsubsection*{Part C}

$Y = e^X$

\noindent $f_X(x) = \frac{1}{\sigma^2} x e^{-(x/\sigma)/2}$, $0 < x < \infty$, $\sigma^2$ is a positive constant.

\noindent Solve for $g^{-1}(y)$

\begin{align*}
	y &= e^x \\
	ln(y) &= x \\
	g^{-1}(y) &= ln(y)
\end{align*}

\noindent Derivative of $g^{-1}(y)$

\begin{align*}
	\frac{d}{dy} g^{-1}(y) &= \frac{d}{dy} ln(y) \\
	&= \frac{1}{y}
\end{align*}

Range of Y: $\mathcal{Y} = (0, \infty)$

Put it all together

\[
	f_X(g^{-1}(y)) \cdot \left| \frac{d}{dy} g^{-1}(y) \right| = \frac{1}{\sigma^2} ln(y) e^{-(ln(y)/\sigma)/2} \cdot \left| \frac{1}{y} \right|
\]

\[
	f_Y(y) = \begin{cases}
		\frac{1}{\sigma^2} ln(y) e^{-(ln(y)/\sigma)/2} \cdot \frac{1}{y} & 0 < y < \infty \\
		0 & o/w
	\end{cases}
\]
